Indent code + grammer fixes

managerOnlyUpdates - with changes.dfy
@@ -42,13 +42,13 @@ class AdvertisingManager {
         ads := adService.removeAdOfPublisher(publisher, ads);
     }
 
-    method startPublish (publisher : Publisher, price : int)
+    method startPublish (publisher : Publisher, rentPrice : int)
     modifies this
     modifies adService
     requires startPublishRequirements(publisher, availableBanners, publishers, ads)
     requires isNoNull (availableBanners, publishers, ads) &&  adService != null
     {
-        publishers, ads, availableBanners := adService.startPublish(publisher, price, publishers, ads, availableBanners);
+        publishers, ads, availableBanners := adService.startPublish(publisher, rentPrice, publishers, ads, availableBanners);
     }
 
     method isPublishing(publisher : Publisher) returns (status : bool)
@@ -61,7 +61,7 @@ class AdvertisingManager {
     method isBannerAvailable(banner : Banner) returns (status : bool)
     ensures banner in availableBanners <==> status == true
     {
-        return banner in availableBanners;
+		return banner in availableBanners;
     }
 }
 
@@ -88,8 +88,9 @@ class AdvertisingService
     {
         var index := 0;
         var newBanners : seq<Banner> := [];
+		
         while (index < |availableBanners|)
-            decreases |availableBanners| - index
+        decreases |availableBanners| - index
         invariant removeBannerLoopInvariant(index, availableBanners, newBanners, banner)
         {
             if (availableBanners[index] != banner)
@@ -112,8 +113,9 @@ class AdvertisingService
     {
         var index := 0;
         var newPublishers : seq<Publisher> := [];
+		
         while (index < |publishers|)
-            decreases |publishers| - index
+        decreases |publishers| - index
         invariant removePublisherLoopInvariant(index, publishers, newPublishers, publisher)
         {
             if (publishers[index] != publisher)
@@ -122,7 +124,6 @@ class AdvertisingService
             }
             index := index + 1;
         }
-
         return newPublishers;
     }
 
@@ -132,11 +133,11 @@ class AdvertisingService
         return publishers + [publisher];
     }
 
-    method addAd (publisher : Publisher, price : int, banner : Banner, ads : map <Publisher, Ad>) returns (retAds : map <Publisher, Ad>)
+    method addAd (publisher : Publisher, rentPrice : int, banner : Banner, ads : map <Publisher, Ad>) returns (retAds : map <Publisher, Ad>)
     requires banner != null
-    ensures addAdInvariant(publisher, price, banner, retAds)
+    ensures addAdInvariant(publisher, rentPrice, banner, retAds)
     {
-        var newAd : Ad := new Ad(banner, price);
+        var newAd : Ad := new Ad(banner, rentPrice);
         return ads[publisher := newAd];
     }
 
@@ -152,14 +153,14 @@ class AdvertisingService
     ensures minPublisherFound(retPrice, retPublisher, publishers, ads)
     {
         var minPublisher := publishers[0];
-        var minPrice := ads[minPublisher].price;
+        var minPrice := ads[minPublisher].rentPrice;
 
         var index := 1;
         while (index < |publishers|)
-            decreases |publishers| - index
+        decreases |publishers| - index
         invariant findMinPublisherLoopInvariant(minPrice, ads, index, publishers, minPublisher)
         {
-            var curPrice := ads[publishers[index]].price;
+            var curPrice := ads[publishers[index]].rentPrice;
             if (curPrice < minPrice)
             {
                 minPrice := curPrice;
@@ -170,11 +171,11 @@ class AdvertisingService
         return minPublisher, minPrice;
     }
 
-    method startPublish(publisher : Publisher, price : int, publishers : seq<Publisher>, ads : map <Publisher, Ad>, availableBanners : seq<Banner>) returns (retPublishers : seq<Publisher>, retAds : map <Publisher, Ad>, retBanners : seq<Banner>)
+    method startPublish(publisher : Publisher, rentPrice : int, publishers : seq<Publisher>, ads : map <Publisher, Ad>, availableBanners : seq<Banner>) returns (retPublishers : seq<Publisher>, retAds : map <Publisher, Ad>, retBanners : seq<Banner>)
     modifies this
     requires startPublishRequirements(publisher, availableBanners, publishers, ads)
     requires isNoNull (availableBanners, publishers, ads)
-    ensures startPublishInvariant(publisher, price, publishers, retPublishers, ads, retAds, availableBanners, retBanners, globalMinPublisher)
+    ensures startPublishInvariant(publisher, rentPrice, publishers, retPublishers, ads, retAds, availableBanners, retBanners, globalMinPublisher)
     {
         var newPublishers : seq<Publisher> := publishers;
         var newAds : map <Publisher, Ad> := ads;
@@ -183,26 +184,25 @@ class AdvertisingService
         if (|availableBanners| > 0)
         {
             newPublishers := addPublisher(publisher, newPublishers);
-            newAds := addAd(publisher, price, newBanners[0], newAds);
+            newAds := addAd(publisher, rentPrice, newBanners[0], newAds);
             newBanners := popFirstBanner(newBanners);
         }
-      else
+        else
         {
             if (|newPublishers| > 0)
             {
                 var minPublisher, minPrice := findMinPublisher(newPublishers, newAds);
                 globalMinPublisher := minPublisher;
-                if (price > minPrice)
+                if (rentPrice > minPrice)
                 {
                     var banner := newAds[minPublisher].banner;
-                    newAds := addAd(publisher, price, banner, newAds);
+                    newAds := addAd(publisher, rentPrice, banner, newAds);
                     newAds := removeAdOfPublisher(minPublisher, newAds);
                     newPublishers := addPublisher(publisher, newPublishers);
                     newPublishers := removePublisher(minPublisher, newPublishers);
                 }
             }
         }
-
         return newPublishers, newAds, newBanners;
     }
 
@@ -231,245 +231,240 @@ class Banner
 class Ad
 {
     var banner : Banner;
-    var price : int;
+    var rentPrice : int;
 
     constructor(bannerArg : Banner, priceArg : int)
     modifies this
     requires bannerArg != null
-    ensures banner == bannerArg && price == priceArg
+    ensures banner == bannerArg && rentPrice == priceArg
     {
         banner := bannerArg;
-        price := priceArg;
+        rentPrice := priceArg;
     }
 }
 
 // Conditions Functions
 
-    function isPublishing (publisher : Publisher, ads: map <Publisher, Ad>, publishers : seq<Publisher>) : bool
-        {
-        publisher !in publishers &&
-        publisher !in ads
-        }
+function isPublishing (publisher : Publisher, ads: map <Publisher, Ad>, publishers : seq<Publisher>) : bool
+{
+    publisher !in publishers &&
+    publisher !in ads
+}
 
-        function adsKeysEqualsPublishers (ads: map <Publisher, Ad>, publishers : seq<Publisher>) : bool
-        {
-        (forall p :: p in publishers ==> p in ads) &&
-        (forall p :: p in ads ==> p in publishers)
-        }
+function adsKeysEqualsPublishers (ads: map <Publisher, Ad>, publishers : seq<Publisher>) : bool
+{
+	(forall p :: p in publishers ==> p in ads) &&
+    (forall p :: p in ads ==> p in publishers)
+}
 
-        function valuesOfAds (myAds : map<Publisher, Ad>) : set<Ad>
-        {
-                set p: Publisher | p in myAds :: myAds[p]
-                }
+function valuesOfAds (myAds : map<Publisher, Ad>) : set<Ad>
+{
+	set p: Publisher | p in myAds :: myAds[p]
+}
 
-                function isNoNullPublishers (ads: map <Publisher, Ad>, publishers : seq<Publisher>) : bool
-        requires adsKeysEqualsPublishers(ads, publishers)
-        reads valuesOfAds(ads)
-        {
-        forall p :: p in publishers ==> p != null && ads[p] != null && ads[p].banner != null
-        }
+function isNoNullPublishers (ads: map <Publisher, Ad>, publishers : seq<Publisher>) : bool
+requires adsKeysEqualsPublishers(ads, publishers)
+reads valuesOfAds(ads)
+{
+    forall p :: p in publishers ==> p != null && ads[p] != null && ads[p].banner != null
+}
 
-        function isNoNullAds (ads: map <Publisher, Ad>) : bool
-        {
-        forall p :: p in ads ==> ads[p] != null
-        }
+function isNoNullAds (ads: map <Publisher, Ad>) : bool
+{
+    forall p :: p in ads ==> ads[p] != null
+}
 
-        function isNoNullAvailableBanners (availableBanners: seq<Banner>) : bool
-        {
-        forall i :: 0 <= i < |availableBanners| ==> availableBanners[i] != null
-        }
+function isNoNullAvailableBanners (availableBanners: seq<Banner>) : bool
+{
+	forall i :: 0 <= i < |availableBanners| ==> availableBanners[i] != null
+}
 
-        function isUniqueAvailableBanners (availableBanners: seq<Banner>) : bool
-        {
-        |availableBanners| > 0 ==> availableBanners[0] !in availableBanners[1..]
-        }
+function isUniqueAvailableBanners (availableBanners: seq<Banner>) : bool
+{
+	|availableBanners| > 0 ==> availableBanners[0] !in availableBanners[1..]
+}
 
-        function isPublisherInAds (publisher : Publisher, retAds: map <Publisher, Ad>) : bool
-        {
-        publisher in retAds &&
-        retAds[publisher] != null
-        }
+function isPublisherInAds (publisher : Publisher, retAds: map <Publisher, Ad>) : bool
+{
+	publisher in retAds &&
+	retAds[publisher] != null
+}
 
-        function startPublishWithAvailableBanner(publisher : Publisher, price : int, publishers : seq<Publisher>, retPublishers: seq<Publisher>, ads : map <Publisher, Ad>, retAds: map <Publisher, Ad>, availableBanners : seq<Banner>, retBanners: seq<Banner>) : bool
-        reads valuesOfAds(retAds)
-        {
-        |availableBanners| > 0 ==> publisher in retPublishers &&
-        publisher in retAds &&
-        retAds[publisher] != null &&
-        retAds[publisher].price == price  &&
-        availableBanners[0] == retAds[publisher].banner &&
-        retBanners == availableBanners[1..] &&
-        availableBanners[0] !in retBanners
-        }
+function startPublishWithAvailableBanner(publisher : Publisher, rentPrice : int, publishers : seq<Publisher>, retPublishers: seq<Publisher>, ads : map <Publisher, Ad>, retAds: map <Publisher, Ad>, availableBanners : seq<Banner>, retBanners: seq<Banner>) : bool
+reads valuesOfAds(retAds)
+{
+	|availableBanners| > 0 ==> publisher in retPublishers &&
+	publisher in retAds &&
+	retAds[publisher] != null &&
+	retAds[publisher].rentPrice == rentPrice  &&
+	availableBanners[0] == retAds[publisher].banner &&
+	retBanners == availableBanners[1..] &&
+	availableBanners[0] !in retBanners
+}
 
-        function startPublishEmptyList (publisher : Publisher, price : int, publishers : seq<Publisher>, retPublishers: seq<Publisher>, ads : map <Publisher, Ad>, retAds: map <Publisher, Ad>, availableBanners : seq<Banner>, retBanners: seq<Banner>) : bool
-        {
-        (|availableBanners| == 0 &&
-        |publishers| == 0) ==> publishers == retPublishers &&
-        ads == retAds &&
-        availableBanners == retBanners &&
-        publisher !in publishers &&
-        publisher !in ads
-        }
+function startPublishEmptyList (publisher : Publisher, rentPrice : int, publishers : seq<Publisher>, retPublishers: seq<Publisher>, ads : map <Publisher, Ad>, retAds: map <Publisher, Ad>, availableBanners : seq<Banner>, retBanners: seq<Banner>) : bool
+{
+	(|availableBanners| == 0 &&
+	|publishers| == 0) ==> publishers == retPublishers &&
+	ads == retAds &&
+	availableBanners == retBanners &&
+	publisher !in publishers &&
+	publisher !in ads
+}
 
-        function publishingStarted (publisher : Publisher, price : int, publishers : seq<Publisher>, retPublishers: seq<Publisher>, ads : map <Publisher, Ad>, retAds: map <Publisher, Ad>, availableBanners : seq<Banner>, retBanners: seq<Banner>, globalMinPublisher: Publisher) : bool
-        reads valuesOfAds(retAds)
-        reads valuesOfAds(ads)
-        requires forall p :: p in ads ==> ads[p] != null
-        {
-        (|availableBanners| == 0 &&
-        |publishers| > 0 &&
-        !isPriceLessThanMinPrice(price, ads)) ==> (publisher in retPublishers &&
-        isPublisherInAds(publisher, retAds) &&
-        retAds[publisher].price == price &&
-        availableBanners == retBanners) &&
-        (globalMinPublisher !in retPublishers &&
-        globalMinPublisher !in retAds &&
-        globalMinPublisher in ads &&
-        retAds[publisher].banner == ads[globalMinPublisher].banner)
-        }
+function publishingStarted (publisher : Publisher, rentPrice : int, publishers : seq<Publisher>, retPublishers: seq<Publisher>, ads : map <Publisher, Ad>, retAds: map <Publisher, Ad>, availableBanners : seq<Banner>, retBanners: seq<Banner>, globalMinPublisher: Publisher) : bool
+reads valuesOfAds(retAds)
+reads valuesOfAds(ads)
+requires forall p :: p in ads ==> ads[p] != null
+{
+	(|availableBanners| == 0 &&
+	|publishers| > 0 &&
+	!isPriceLessThanMinPrice(rentPrice, ads)) ==> (publisher in retPublishers &&
+	isPublisherInAds(publisher, retAds) &&
+	retAds[publisher].rentPrice == rentPrice &&
+	availableBanners == retBanners) &&
+	(globalMinPublisher !in retPublishers &&
+	globalMinPublisher !in retAds &&
+	globalMinPublisher in ads &&
+	retAds[publisher].banner == ads[globalMinPublisher].banner)
+}
 
-        function isPriceLessThanMinPrice (price : int, ads: map <Publisher, Ad>) : bool
-        reads valuesOfAds(ads)
-        {
-        forall p :: p in ads &&
-        ads[p] != null ==> ads[p].price >= price
-        }
+function isPriceLessThanMinPrice (rentPrice : int, ads: map <Publisher, Ad>) : bool
+reads valuesOfAds(ads)
+{
+	forall p :: p in ads &&
+	ads[p] != null ==> ads[p].rentPrice >= rentPrice
+}
 
-        function publishingNotStarted (publisher : Publisher, price : int, publishers : seq<Publisher>, retPublishers: seq<Publisher>, ads : map <Publisher, Ad>, retAds: map <Publisher, Ad>, availableBanners : seq<Banner>, retBanners: seq<Banner>) : bool
-        reads valuesOfAds(ads)
-        {
-        (|availableBanners| == 0 &&
-        |publishers| > 0 &&
-        isPriceLessThanMinPrice(price, ads)) ==> publishers == retPublishers &&
-        ads == retAds && availableBanners == retBanners &&
-        isPublishing(publisher, ads, publishers)
-        }
+function publishingNotStarted (publisher : Publisher, rentPrice : int, publishers : seq<Publisher>, retPublishers: seq<Publisher>, ads : map <Publisher, Ad>, retAds: map <Publisher, Ad>, availableBanners : seq<Banner>, retBanners: seq<Banner>) : bool
+reads valuesOfAds(ads)
+{
+	(|availableBanners| == 0 &&
+	|publishers| > 0 &&
+	isPriceLessThanMinPrice(rentPrice, ads)) ==> publishers == retPublishers &&
+	ads == retAds && availableBanners == retBanners &&
+	isPublishing(publisher, ads, publishers)
+}
 
-        function isNoNull (availableBanners: seq<Banner>, publishers : seq<Publisher>, ads : map <Publisher, Ad>)  : bool
-        reads valuesOfAds(ads)
-        requires adsKeysEqualsPublishers(ads, publishers)
-        {
-        isNoNullPublishers(ads,publishers) &&
-        isNoNullAds(ads) &&
-        isNoNullAvailableBanners(availableBanners)
-        }
+function isNoNull (availableBanners: seq<Banner>, publishers : seq<Publisher>, ads : map <Publisher, Ad>)  : bool
+reads valuesOfAds(ads)
+requires adsKeysEqualsPublishers(ads, publishers)
+{
+	isNoNullPublishers(ads,publishers) &&
+	isNoNullAds(ads) &&
+	isNoNullAvailableBanners(availableBanners)
+}
 
-        function adExists(adService : AdvertisingService, publisher: Publisher, ads: map <Publisher, Ad>, availableBanners: seq<Banner>) : bool
-        reads valuesOfAds(ads)
-        {
-        isPublisherInAds(publisher, ads) &&
-        ads[publisher].banner !in availableBanners
-        }
+function adExists(adService : AdvertisingService, publisher: Publisher, ads: map <Publisher, Ad>, availableBanners: seq<Banner>) : bool
+reads valuesOfAds(ads)
+{
+	isPublisherInAds(publisher, ads) &&
+	ads[publisher].banner !in availableBanners
+}
 
-        function startPublishRequirements (publisher: Publisher, availableBanners: seq<Banner>, publishers : seq<Publisher>, ads : map <Publisher, Ad>)  : bool
-        reads valuesOfAds(ads)
-        {
-        isPublishing(publisher, ads, publishers) &&
-        adsKeysEqualsPublishers(ads, publishers) &&
-        isUniqueAvailableBanners(availableBanners) &&
-        adsKeysEqualsPublishers(ads, publishers)
-        }
+function startPublishRequirements (publisher: Publisher, availableBanners: seq<Banner>, publishers : seq<Publisher>, ads : map <Publisher, Ad>)  : bool
+reads valuesOfAds(ads)
+{
+	isPublishing(publisher, ads, publishers) &&
+	adsKeysEqualsPublishers(ads, publishers) &&
+	isUniqueAvailableBanners(availableBanners) &&
+	adsKeysEqualsPublishers(ads, publishers)
+}
 
-        function findMinPublisherRequirements(publishers : seq<Publisher>, ads : map <Publisher, Ad>) : bool
-        reads valuesOfAds(ads)
-        {
-        |publishers| > 0 &&
-        forall p :: p in publishers ==> p != null &&
-        p in ads && ads[p] != null &&
-        ads[p].banner != null &&
-        adsKeysEqualsPublishers(ads, publishers) &&
-        isNoNullAds(ads) &&
-        (forall p :: p in ads ==> ads[p] != null)
-        }
+function findMinPublisherRequirements(publishers : seq<Publisher>, ads : map <Publisher, Ad>) : bool
+reads valuesOfAds(ads)
+{
+	|publishers| > 0 &&
+	forall p :: p in publishers ==> p != null &&
+	p in ads && ads[p] != null &&
+	ads[p].banner != null &&
+	adsKeysEqualsPublishers(ads, publishers) &&
+	isNoNullAds(ads) &&
+	(forall p :: p in ads ==> ads[p] != null)
+}
 
-        function minPublisherFound(retPrice : int, retPublisher : Publisher, publishers : seq<Publisher>, ads : map <Publisher, Ad>) : bool
-        requires findMinPublisherRequirements(publishers, ads)
-        reads valuesOfAds(ads)
-        {
-        retPublisher in ads &&
-        retPublisher in publishers &&
-        retPublisher != null &&
-        ads[retPublisher] != null &&
-        ads[retPublisher].banner != null &&
-        ads[retPublisher].price == retPrice &&
-        forall p :: p in ads ==> ads[p].price >= retPrice
-        }
+function minPublisherFound(retPrice : int, retPublisher : Publisher, publishers : seq<Publisher>, ads : map <Publisher, Ad>) : bool
+requires findMinPublisherRequirements(publishers, ads)
+reads valuesOfAds(ads)
+{
+	retPublisher in ads &&
+	retPublisher in publishers &&
+	retPublisher != null &&
+	ads[retPublisher] != null &&
+	ads[retPublisher].banner != null &&
+	ads[retPublisher].rentPrice == retPrice &&
+	forall p :: p in ads ==> ads[p].rentPrice >= retPrice
+}
 
-        function startPublishInvariant(publisher : Publisher, price : int, publishers : seq<Publisher>, retPublishers: seq<Publisher>, ads : map <Publisher, Ad>, retAds: map <Publisher, Ad>, availableBanners : seq<Banner>, retBanners: seq<Banner>, globalMinPublisher: Publisher) : bool
-        reads valuesOfAds(retAds)
-        reads valuesOfAds(ads)
-        requires forall p :: p in ads ==> ads[p] != null
-        {
-        startPublishWithAvailableBanner(publisher, price, publishers, retPublishers, ads, retAds, availableBanners, retBanners) &&
-        publishingNotStarted(publisher, price, publishers, retPublishers, ads, retAds, availableBanners, retBanners) &&
-        publishingStarted(publisher, price, publishers, retPublishers, ads, retAds, availableBanners, retBanners, globalMinPublisher) &&
-        startPublishEmptyList(publisher, price, publishers, retPublishers, ads, retAds, availableBanners, retBanners)
-        }
+function startPublishInvariant(publisher : Publisher, rentPrice : int, publishers : seq<Publisher>, retPublishers: seq<Publisher>, ads : map <Publisher, Ad>, retAds: map <Publisher, Ad>, availableBanners : seq<Banner>, retBanners: seq<Banner>, globalMinPublisher: Publisher) : bool
+reads valuesOfAds(retAds)
+reads valuesOfAds(ads)
+requires forall p :: p in ads ==> ads[p] != null
+{
+	startPublishWithAvailableBanner(publisher, rentPrice, publishers, retPublishers, ads, retAds, availableBanners, retBanners) &&
+	publishingNotStarted(publisher, rentPrice, publishers, retPublishers, ads, retAds, availableBanners, retBanners) &&
+	publishingStarted(publisher, rentPrice, publishers, retPublishers, ads, retAds, availableBanners, retBanners, globalMinPublisher) &&
+	startPublishEmptyList(publisher, rentPrice, publishers, retPublishers, ads, retAds, availableBanners, retBanners)
+}
 
-        function removePublisherLoopInvariant(index: int, publishers: seq<Publisher>, newPublishers: seq<Publisher>, publisher: Publisher) : bool
-        {
-        0 <= index <= |publishers| &&
-        publisher !in newPublishers &&
-        forall i :: 0 <= i < index &&
-        publishers[i] != publisher ==> publishers[i] in newPublishers
-        }
+function removePublisherLoopInvariant(index: int, publishers: seq<Publisher>, newPublishers: seq<Publisher>, publisher: Publisher) : bool
+{
+	0 <= index <= |publishers| &&
+	publisher !in newPublishers &&
+	forall i :: 0 <= i < index &&
+	publishers[i] != publisher ==> publishers[i] in newPublishers
+}
 
+function findMinPublisherLoopInvariant(minPrice: int, ads : map <Publisher, Ad>, index: int, publishers: seq<Publisher>, minPublisher: Publisher) : bool
+requires isNoNullAds(ads)
+requires adsKeysEqualsPublishers(ads, publishers)
+reads valuesOfAds(ads)
+{
+	forall p :: p in publishers ==> p in ads &&
+	minPublisher in ads &&
+	ads[minPublisher] != null &&
+	ads[minPublisher].rentPrice == minPrice &&
+	minPublisher in publishers &&
+	0 <= index <= |publishers| &&
+	minPublisher in ads &&
+	forall i :: 0 <= i < index ==> minPrice <= ads[publishers[i]].rentPrice &&
+	isNoNullAds(ads)
+}
 
-        function findMinPublisherLoopInvariant(minPrice: int, ads : map <Publisher, Ad>, index: int, publishers: seq<Publisher>, minPublisher: Publisher) : bool
-        requires isNoNullAds(ads)
-        requires adsKeysEqualsPublishers(ads, publishers)
-        reads valuesOfAds(ads)
-        {
-        forall p :: p in publishers ==> p in ads &&
-        minPublisher in ads &&
-        ads[minPublisher] != null &&
-        ads[minPublisher].price == minPrice &&
-        minPublisher in publishers &&
-        0 <= index <= |publishers| &&
-        minPublisher in ads &&
-        forall i :: 0 <= i < index ==> minPrice <= ads[publishers[i]].price &&
-        isNoNullAds(ads)
-        }
+function bannerRemovedInvariant(banner : Banner, retBanners : seq<Banner>, availableBanners : seq<Banner>) : bool
+{
+	banner !in retBanners &&
+	forall b :: b in availableBanners && b != banner ==> b in retBanners
+}
 
-        function bannerRemovedInvariant(banner : Banner, retBanners : seq<Banner>, availableBanners : seq<Banner>) : bool
-        {
-        banner !in retBanners &&
-        forall b :: b in availableBanners && b != banner ==> b in retBanners
-        }
+function adRemovedInvariant(publisher : Publisher, retAds : map <Publisher, Ad>, ads : map <Publisher, Ad>) : bool
+{
+	publisher !in retAds &&
+	forall p :: p in ads && p != publisher ==> p in retAds && retAds[p] == ads[p]
+}
 
-        function adRemovedInvariant(publisher : Publisher, retAds : map <Publisher, Ad>, ads : map <Publisher, Ad>) : bool
-        {
-        publisher !in retAds &&
-        forall p :: p in ads && p != publisher ==> p in retAds && retAds[p] == ads[p]
-        }
+function removePublisherInvariant(publisher : Publisher, publishers : seq<Publisher>, retPublishers : seq<Publisher>) : bool
+{
+	publisher !in retPublishers &&
+	forall p :: p in publishers &&
+	p != publisher ==> p in retPublishers
+}
 
-        function removePublisherInvariant(publisher : Publisher, publishers : seq<Publisher>, retPublishers : seq<Publisher>) : bool
-        {
-        publisher !in retPublishers &&
-        forall p :: p in publishers &&
-        p != publisher ==> p in retPublishers
-        }
+function addPublisherInvariant(publisher : Publisher, publishers : seq<Publisher>, retPublishers : seq<Publisher>) : bool
+{
+	publisher in retPublishers &&
+	forall p :: p in publishers ==> p in retPublishers
+}
 
-        function addPublisherInvariant(publisher : Publisher, publishers : seq<Publisher>, retPublishers : seq<Publisher>) : bool
-        {
-        publisher in retPublishers &&
-        forall p :: p in publishers ==> p in retPublishers
-        }
+function addAdInvariant(publisher : Publisher, rentPrice : int, banner : Banner, retAds : map <Publisher, Ad>) : bool
+reads valuesOfAds(retAds)
+{
+	isPublisherInAds(publisher, retAds) &&
+	retAds[publisher].rentPrice == rentPrice &&
+	retAds[publisher].banner == banner
+}
 
-        function addAdInvariant(publisher : Publisher, price : int, banner : Banner, retAds : map <Publisher, Ad>) : bool
-        reads valuesOfAds(retAds)
-        {
-        isPublisherInAds(publisher, retAds) &&
-        retAds[publisher].price == price &&
-        retAds[publisher].banner == banner
-        }
-
-        function removeBannerLoopInvariant(index: int, availableBanners: seq<Banner>, newBanners: seq<Banner>, banner: Banner) : bool
-        {
-        0 <= index <= |availableBanners| && banner !in newBanners && forall i :: 0 <= i < index && availableBanners[i] != banner ==> availableBanners[i] in newBanners
-        }
-
-
-
-
+function removeBannerLoopInvariant(index: int, availableBanners: seq<Banner>, newBanners: seq<Banner>, banner: Banner) : bool
+{
+	0 <= index <= |availableBanners| && banner !in newBanners && forall i :: 0 <= i < index && availableBanners[i] != banner ==> availableBanners[i] in newBanners
+}
